coq/ptt.v
@@ -1,7 +1,7 @@
 Require Export Setoid Morphisms.
 From mathcomp Require Import all_ssreflect.
 Require Import edone preliminaries.
-Require Export structures.
+Require Export structures pttdom.
 
 Set Implicit Arguments.
 Unset Strict Implicit.
@@ -12,66 +12,53 @@ Set Bullet Behavior "Strict Subproofs".
 
 (** ** 2p algebras (2pdom algebras with top) *)
 
-(* TODO: prove that 2p-algebras are 2pdom algebras to share related definitions and proofs 
-   (requires properly setting up structures)
- *)
-
-(* operations are put apart so that the can get notations for them before stating/proving the laws  *)
-Structure ops_ :=
-  { setoid_of_ops:> setoid;
-    dot: setoid_of_ops -> setoid_of_ops -> setoid_of_ops;
-    par: setoid_of_ops -> setoid_of_ops -> setoid_of_ops;
-    cnv: setoid_of_ops -> setoid_of_ops;
-    dom: setoid_of_ops -> setoid_of_ops;
-    one: setoid_of_ops;
-    top: setoid_of_ops }.
-
-(* Declare Scope ptt_ops. compat:coq-8.9*)
-Bind Scope ptt_ops with setoid_of_ops.
-Delimit Scope ptt_ops with ptt.
-Open Scope ptt_ops.
-Notation "x ∥ y" := (par x y) (left associativity, at level 40, format "x ∥ y"): ptt_ops.
-Notation "x · y" := (dot x y) (left associativity, at level 25, format "x · y"): ptt_ops.
-Notation "x °"  := (cnv x) (left associativity, at level 5, format "x °"): ptt_ops.
-Notation "1"  := (one _): ptt_ops.
-Arguments top {_}.
-
 (* 2p axioms *)
 Structure ptt :=
   { ops:> ops_;
-    dot_eqv: Proper (eqv ==> eqv ==> eqv) (@dot ops);
-    par_eqv: Proper (eqv ==> eqv ==> eqv) (@par ops);
-    cnv_eqv: Proper (eqv ==> eqv) (@cnv ops);
+    dot_eqv_: Proper (eqv ==> eqv ==> eqv) (@dot ops);
+    par_eqv_: Proper (eqv ==> eqv ==> eqv) (@par ops);
+    cnv_eqv_: Proper (eqv ==> eqv) (@cnv ops);
     domE: forall x: ops, dom x ≡ 1 ∥ x·top;
-    parA: forall x y z: ops, x ∥ (y ∥ z) ≡ (x ∥ y) ∥ z;
-    parC: forall x y: ops, x ∥ y ≡ y ∥ x;
-    dotA: forall x y z: ops, x · (y · z) ≡ (x · y) · z;
-    dotx1: forall x: ops, x · 1 ≡ x;
-    cnvI: forall x: ops, x°° ≡ x;
-    cnvpar: forall x y: ops, (x ∥ y)° ≡ x° ∥ y°;
-    cnvdot: forall x y: ops, (x · y)° ≡ y° · x°;
-    par11: 1 ∥ 1 ≡ one ops;
-    A10: forall x y: ops, 1 ∥ x·y ≡ dom (x ∥ y°);
+    parA_: forall x y z: ops, x ∥ (y ∥ z) ≡ (x ∥ y) ∥ z;
+    parC_: forall x y: ops, x ∥ y ≡ y ∥ x;
+    dotA_: forall x y z: ops, x · (y · z) ≡ (x · y) · z;
+    dotx1_: forall x: ops, x · 1 ≡ x;
+    cnvI_: forall x: ops, x°° ≡ x;
+    cnvpar_: forall x y: ops, (x ∥ y)° ≡ x° ∥ y°;
+    cnvdot_: forall x y: ops, (x · y)° ≡ y° · x°;
+    par11_: 1 ∥ 1 ≡ @one ops;
+    A10_: forall x y: ops, 1 ∥ x·y ≡ dom (x ∥ y°);
     A11: forall x: ops, x · top ≡ dom x · top;
     A12: forall x y: ops, (x∥1) · y ≡ (x∥1)·top ∥ y
   }.
-Existing Instances dot_eqv par_eqv cnv_eqv.
 
 (** ** basic derivable laws  *)
 Section derived.
  Variable X: ptt.
+ Existing Instances dot_eqv_ par_eqv_ cnv_eqv_.
   
- Global Instance dom_eqv: Proper (eqv ==> eqv) (@dom X).
+ Instance dom_eqv_: Proper (eqv ==> eqv) (@dom X).
  Proof. intros ?? H. by rewrite 2!domE H. Qed.
+ 
+ Lemma A13_ (x y: X): dom(x·y) ≡ dom(x·dom y).
+ Proof. by rewrite domE -dotA_ A11 dotA_ -domE. Qed.
 
- Lemma cnv1: 1° ≡ @one X.
- Proof.
-  rewrite -(dotx1 1°) -{2}(cnvI 1).
-  by rewrite -cnvdot dotx1 cnvI.
- Qed.
+ Lemma A14_ (x y z: X): dom x·(y∥z) ≡ dom x·y ∥ z.
+ Proof. by rewrite domE parC_ A12 (A12 _ y) parA_. Qed.
 
- Lemma dot1x (x: X): 1·x ≡ x.
- Proof. by rewrite -(cnvI (1·x)) cnvdot cnv1 dotx1 cnvI. Qed.
+ Program Definition pttdom_of: pttdom := {| pttdom.ops := ops X |}.
+ Next Obligation. apply parA_. Qed.
+ Next Obligation. apply parC_. Qed.
+ Next Obligation. apply dotA_. Qed.
+ Next Obligation. apply dotx1_. Qed.
+ Next Obligation. apply cnvI_. Qed.
+ Next Obligation. apply cnvpar_. Qed.
+ Next Obligation. apply cnvdot_. Qed.
+ Next Obligation. apply par11_. Qed.
+ Next Obligation. apply A10_. Qed.
+ Next Obligation. apply A13_. Qed.
+ Next Obligation. apply A14_. Qed.
+ Canonical pttdom_of. 
 
  Lemma parxtop (x: X): x ∥ top ≡ x.
  Proof.
@@ -88,117 +75,7 @@ Section derived.
   by rewrite -cnvpar partopx cnvI.
  Qed.
 
- Lemma cnv_inj (x y: X): x° ≡ y° -> x ≡ y.
- Proof. intro H. by rewrite -(cnvI x) -(cnvI y) H. Qed.
-
- Lemma dotcnv (x y: X): x·y ≡ (y°·x°)°.
- Proof. apply cnv_inj. by rewrite cnvdot cnvI. Qed.
- 
- Lemma A13 (x y: X): dom(x·y) ≡ dom(x·dom y).
- Proof. by rewrite domE -dotA A11 dotA -domE. Qed.
-
- Lemma A14 (x y z: X): dom x·(y∥z) ≡ dom x·y ∥ z.
- Proof. by rewrite domE parC A12 (A12 _ y) parA. Qed.
-
- (** ** tests *)
- Definition is_test (x: X) := dom x ≡ x.
- Record test := Test{ elem_of:> X ; testE: is_test elem_of }.
-
- Lemma is_test_alt (x: X): dom x ≡ x <-> x∥1 ≡ x.
- Proof.
-   split=>E.
-   - rewrite -{1}E -{1}(dotx1 (dom x)) -A14.
-     by rewrite par11 dotx1. 
-   - by rewrite -E -{1}cnv1 -A10 dotx1 parC.
- Qed.
- 
- Lemma domtst (a : test) : dom a ≡ a. 
- Proof. apply testE. Qed.
- 
- Lemma tstpar1 (a : test) : a ∥ 1 ≡ a.
- Proof. apply is_test_alt, domtst. Qed.
-
- Lemma one_test: is_test 1. 
- Proof. rewrite /is_test. by rewrite -{1}par11 -{2}cnv1 -A10 dotx1 par11. Qed.
- Canonical Structure tst_one := Test one_test. 
-
- Lemma dom_test x: is_test (dom x). 
- Proof. rewrite /is_test. by rewrite -{1}[dom x]dot1x -A13 dot1x. Qed.
- Canonical Structure tst_dom x := Test (dom_test x).
- 
- Lemma par_test (a: test) (u: X): is_test (a∥u).
- Proof.
-   rewrite /is_test is_test_alt.
-   by rewrite -parA (parC u) parA tstpar1. 
- Qed.
- Canonical Structure tst_par a u := Test (par_test a u).
-
- Lemma cnvtst (a: test): a° ≡ a.
- Proof.
-   rewrite -tstpar1 cnvpar cnv1 -(dot1x (a°)) parC A10 cnvI parC.
-   apply domtst.
- Qed.
-
- Lemma cnv_test (a: test): is_test (a°).
- Proof.
-   by rewrite /is_test is_test_alt cnvtst tstpar1. 
- Qed.
- Canonical Structure tst_cnv a := Test (cnv_test a).
-
- Lemma tstpar (a: test) (x y: X): a·(x∥y) ≡ a·x ∥ y.
- Proof. rewrite -domtst. apply A14. Qed.
-
- Lemma pardot (a b: test): a ∥ b ≡ a·b.
- Proof.
-   by rewrite -{2}(tstpar1 b) (parC _ 1) tstpar dotx1.
- Qed.
- 
- Lemma dot_test (a b: test): is_test (a·b).
- Proof. rewrite /is_test -pardot. apply domtst. Qed.
- Canonical Structure tst_dot a b := Test (dot_test a b).
- 
- (** automatised inference of tests *)
- Definition infer_test x y (e: elem_of y = x) := y.
- Notation "[ x ]" := (@infer_test x _ erefl).
-
- (** ** commutative monoid of  tests *)
- Definition eqv_test (a b: test) := a ≡ b.
- Arguments eqv_test _ _ /.
- Lemma eqv_test_equiv: Equivalence eqv_test. 
- Proof. 
-   split => [x|x y|x y z]; rewrite /eqv_test /=.
-   reflexivity. by symmetry. by transitivity (elem_of y).
- Qed.
- Canonical Structure ptt_test_setoid := Setoid eqv_test_equiv.
- Lemma tst_dot_eqv: Proper (eqv ==> eqv ==> eqv) tst_dot.
- Proof. intros [a] [b] ? [c] [d] ?. by apply dot_eqv. Qed.
- Lemma tst_dotA: forall a b c: test, a·(b·c) ≡ (a·b)·c.
- Proof. intros [a] [b] [c]. apply dotA. Qed.
- Lemma tst_dotC: forall a b: test, a·b ≡ b·a.
- Proof. intros. rewrite -2!pardot. apply parC. Qed.
- Lemma tst_dotU: forall a: test, a·1 ≡ a.
- Proof. intros [a]. apply dotx1. Qed.
-
- (** ** label structure of a 2pdom algebra (Definition 4.3)  *)
- 
- (* dualised equality (to get the [labels] structure below) *)
- Definition eqv' (x y: X) := x ≡ y°.
- Arguments eqv' _ _ /.
- Lemma eqv'_sym: Symmetric eqv'.
- Proof. move=> x y /= H. apply cnv_inj. by rewrite cnvI H. Qed.
- Lemma eqv01 x y z: x ≡ y -> eqv' y z -> eqv' x z.
- Proof. by move=> /= ->. Qed.
- Lemma eqv11 x y z: eqv' x y -> eqv' y z -> x ≡ z.
- Proof. move=> /= -> ->. apply cnvI. Qed.
- 
- Canonical Structure ptt_labels: labels :=
-   Labels
-     tst_dot_eqv tst_dotA tst_dotC tst_dotU
-     eqv'_sym eqv01 eqv11.
-
 End derived.
-Coercion ptt_labels: ptt >-> labels. 
-Notation "[ x ]" := (@infer_test _ x%ptt _ erefl): ptt_ops.
 
 Arguments eqv : simpl never.
 
@@ -247,23 +124,22 @@ Section terms.
  
  (* quotiented terms indeed form a 2p-algebra *)
  Program Definition tm_ptt: ptt := {| ops := tm_ops_ |}.
- Next Obligation. repeat intro; simpl. by apply dot_eqv. Qed.
- Next Obligation. repeat intro; simpl. by apply par_eqv. Qed.
- Next Obligation. repeat intro; simpl. by apply cnv_eqv. Qed.
+ Next Obligation. repeat intro; simpl. by apply dot_eqv_. Qed.
+ Next Obligation. repeat intro; simpl. by apply par_eqv_. Qed.
+ Next Obligation. repeat intro; simpl. by apply cnv_eqv_. Qed.
  Next Obligation. repeat intro; simpl. by apply domE. Qed.
- Next Obligation. repeat intro; simpl. by apply parA. Qed.
- Next Obligation. repeat intro; simpl. by apply parC. Qed.
- Next Obligation. repeat intro; simpl. by apply dotA. Qed.
- Next Obligation. repeat intro; simpl. by apply dotx1. Qed.
- Next Obligation. repeat intro; simpl. by apply cnvI. Qed.
- Next Obligation. repeat intro; simpl. by apply cnvpar. Qed.
- Next Obligation. repeat intro; simpl. by apply cnvdot. Qed.
- Next Obligation. repeat intro; simpl. by apply par11. Qed.
- Next Obligation. repeat intro; simpl. by apply A10. Qed.
+ Next Obligation. repeat intro; simpl. by apply parA_. Qed.
+ Next Obligation. repeat intro; simpl. by apply parC_. Qed.
+ Next Obligation. repeat intro; simpl. by apply dotA_. Qed.
+ Next Obligation. repeat intro; simpl. by apply dotx1_. Qed.
+ Next Obligation. repeat intro; simpl. by apply cnvI_. Qed.
+ Next Obligation. repeat intro; simpl. by apply cnvpar_. Qed.
+ Next Obligation. repeat intro; simpl. by apply cnvdot_. Qed.
+ Next Obligation. repeat intro; simpl. by apply par11_. Qed.
+ Next Obligation. repeat intro; simpl. by apply A10_. Qed.
  Next Obligation. repeat intro; simpl. by apply A11. Qed.
  Next Obligation. repeat intro; simpl. by apply A12. Qed.
  Canonical tm_ptt. 
- 
- Notation test := (test tm_ptt).
+
 End terms.
 Bind Scope ptt_ops with term.
