coq/transfer.v
@@ -144,7 +144,7 @@ Section PttdomGraphTheory.
 Variable tm : pttdom. 
 Notation test := (test tm).
 
-Notation pre_graph := (pre_graph test (car (setoid_of_ops (ops tm)))).
+Notation pre_graph := (pre_graph test (car (setoid_of_ops (pttdom.ops tm)))).
 Notation graph := (graph (pttdom_labels tm)).
 Notation graph2 := (graph2 (pttdom_labels tm)).
 
